relational spec with memory stores

src/C_strtoimax/AbstractSpec.v
@@ -20,18 +20,18 @@ Definition zero_char := Byte.repr 48.
 Definition is_digit (i : byte) := (Byte.repr 48 <= i) && (i <= Byte.repr 57).
 
 Section ZSpec.
-  
-(* Take a string and a sign and return its integer representation *)
 
-Definition string_to_Z (s : string) :=
+  (* Take a string s and return a pair with its integer representation *)
+
+Definition string_to_Z (s : string) : option Z :=
   let fix string_to_Z_loop s v :=
       match s with
       | [] => v
       | c :: tl =>
         if is_digit c
         then let v := (v * 10 + (Byte.signed c - 48))%Z in
-             string_to_Z_loop tl v
-        else v (* extra stuff is ignored *)     
+             string_to_Z_loop tl v                
+        else v(* extra stuff is ignored *)     
       end
   in match s with
      | nil => None (* not enough data *)
@@ -43,13 +43,181 @@ Definition signed_string_to_Z (s : string) :=
   match s with
   | nil => None 
   | c :: tl => if c == minus_char
-               then option_map Z.opp (string_to_Z tl)
+             then option_map Z.opp (string_to_Z tl)      
                else if c == plus_char
                     then string_to_Z tl
                     else string_to_Z s
   end.
+  
 
 End ZSpec.
+
+
+
+Section RelationalSpec.
+
+  (* To relate the abstract spec we need to add assumption about memory *)
+Definition byte_of_int b := Byte.repr (Int.unsigned b).
+
+(* There is a string s at address str until fin *)
+(* Note: load returns value of type Vint, hence need a conversion from byte *)
+Definition string_at_address m str fin : option (list byte) :=
+  match load_addr Mptr m fin with
+    | Some (Vptr b fin') => 
+      match distance m str (b,fin') with
+      | Some dist =>
+        let fix string_at_address m s str dist : option (list byte) :=
+            match dist with
+            | O => Some s
+            | S n => match load_addr Mint8signed m str with
+                    | Some (Vint i) =>
+                      string_at_address m ((byte_of_int i)::s) (str++) n
+                    | _ => None
+                    end
+            end in
+        string_at_address m nil str dist
+      | _ => None
+      end
+    | _ => None
+  end.
+
+  (* Relational spec without memory stores *)
+  
+  Inductive asn_strtoimax_lim_R m str fin : asn_strtox_result_e -> Prop :=
+    (* Input outside of supported numeric range *)
+  | ASN_STRTOX_ERROR_RANGE_R s z :
+      string_at_address m str fin = Some s ->
+      signed_string_to_Z s = Some z ->
+      (Int64.max_signed <= z)%Z \/ (z <= Int64.min_signed)%Z ->
+      asn_strtoimax_lim_R m str fin ASN_STRTOX_ERROR_RANGE
+    (* Invalid data encountered (e.g., "+-") *)
+  | ASN_STRTOX_ERROR_INVAL_R :
+      addr_ge m str fin = Some true ->
+      asn_strtoimax_lim_R m str fin ASN_STRTOX_ERROR_INVAL
+    (* More data expected (e.g. "+") *)
+  | ASN_STRTOX_EXPECT_MORE_R :
+      string_at_address m str fin = Some [plus_char] \/
+      string_at_address m str fin = Some [minus_char] ->
+      asn_strtoimax_lim_R m str fin ASN_STRTOX_EXPECT_MORE
+    (* Conversion succeded, but the string has extra stuff *)
+  | ASN_STRTOX_EXTRA_DATA_R s z :
+      string_at_address m str fin = Some s ->
+      signed_string_to_Z s = Some z ->
+      (Int64.min_signed <= z <= Int64.max_signed)%Z ->
+      (exists c, In c s /\ is_digit c = false) ->
+      asn_strtoimax_lim_R m str fin ASN_STRTOX_EXTRA_DATA
+      (* Conversion succeded *)
+  | ASN_STRTOX_OK_R s z :
+      string_at_address m str fin = Some s ->
+      signed_string_to_Z s = Some z ->
+      (Int64.min_signed <= z <= Int64.max_signed)%Z ->
+      asn_strtoimax_lim_R m str fin ASN_STRTOX_OK.  
+
+  (* Relational spec with memory stores *)
+  
+  (* We need to store a pointer where we stop in error range, extra data and ok case,
+     hence this additional function:
+
+     Take a string s and an index where either the first non-digit is encountered 
+     or we go out of range. If none of the above happens return (length s) *)
+
+Definition string_to_Z_endpoint (s : string) : option Z :=
+  let fix string_to_Z_loop s v z :=
+      match s with
+      | [] => z
+      | c :: tl =>
+        (* index of c in s *)
+        let i := (Zlength s - (Zlength tl) - 1)%Z in
+        if is_digit c
+        then let v := (v * 10 + (Byte.signed c - 48))%Z in
+             if (Int64.max_signed <=? z)%Z || (z <=? Int64.min_signed)%Z
+             then i
+             else string_to_Z_loop tl v z               
+        else i 
+      end
+  in match s with
+     | nil => None 
+     | _ => Some (string_to_Z_loop s 0%Z (Zlength s))
+     end.
+
+(* The sign is determined by the first char in the string *)
+Definition signed_string_to_Z_endpoint (s : string) :=
+  match s with
+  | nil => None 
+  | c :: tl => if (c == minus_char) || (c == plus_char)
+             then string_to_Z_endpoint tl     
+             else string_to_Z_endpoint s
+  end.
+  
+  Inductive asn_strtoimax_lim_R_mem m str fin intp : mem -> asn_strtox_result_e -> Prop :=
+    (* Input outside of supported numeric range *)
+  | ASN_STRTOX_ERROR_RANGE_R_mem s z m' i :
+      string_at_address m str fin = Some s ->
+      signed_string_to_Z s = Some z ->
+      signed_string_to_Z_endpoint s = Some i ->
+      (Int64.max_signed <= z)%Z \/ (z <= Int64.min_signed)%Z ->
+      store_addr Mptr m fin (vptr (add_addr str (Ptrofs.repr i)))
+      = Some m' -> 
+      asn_strtoimax_lim_R_mem m str fin intp m' ASN_STRTOX_ERROR_RANGE
+    (* Invalid data encountered (e.g., "+-") *)
+  | ASN_STRTOX_ERROR_INVAL_R_mem :
+      addr_ge m str fin = Some true ->
+      asn_strtoimax_lim_R_mem m str fin intp m ASN_STRTOX_ERROR_INVAL
+    (* More data expected (e.g. "+") *)
+  | ASN_STRTOX_EXPECT_MORE_R_mem m':
+      string_at_address m str fin = Some [plus_char] \/
+      string_at_address m str fin = Some [minus_char] ->
+      store_addr Mptr m fin (vptr (str++)) = Some m' -> 
+      asn_strtoimax_lim_R_mem m str fin intp m' ASN_STRTOX_EXPECT_MORE
+    (* Conversion succeded, but the string has extra stuff *)
+  | ASN_STRTOX_EXTRA_DATA_R_mem s z m' m'' i:
+      string_at_address m str fin = Some s ->
+      signed_string_to_Z s = Some z ->
+      signed_string_to_Z_endpoint s = Some i ->
+      (Int64.min_signed <= z <= Int64.max_signed)%Z ->
+      (exists c, In c s /\ is_digit c = false) ->
+      store_addr Mptr m fin (vptr (add_addr str (Ptrofs.repr i)))
+      = Some m' -> 
+      store_addr Mint64 m' intp (Vlong (Int64.repr z)) = Some m'' -> 
+      asn_strtoimax_lim_R_mem m str fin intp m'' ASN_STRTOX_EXTRA_DATA
+      (* Conversion succeded *)
+  | ASN_STRTOX_OK_R_mem s z m' m'':
+      string_at_address m str fin = Some s ->
+      signed_string_to_Z s = Some z ->
+      (Int64.min_signed <= z <= Int64.max_signed)%Z ->
+      store_addr Mptr m fin (vptr (add_addr str (Ptrofs.repr (Zlength s))))
+      = Some m' -> 
+      store_addr Mint64 m' intp (Vlong (Int64.repr z)) = Some m'' -> 
+      asn_strtoimax_lim_R_mem m str fin intp m'' ASN_STRTOX_OK.
+  
+End RelationalSpec.
+
+Theorem asn_strtoimax_lim_func_correct : forall m str fin fin' intp res val p s' m',
+    asn_strtoimax_lim m str fin intp = Some {| return_type := res;
+                                               value := val;
+                                               str_pointer := p;
+                                               memory := Some m';
+                                               sign := s';|}
+    <-> asn_strtoimax_lim_R_mem m str fin' intp m' res.
+Proof.
+  intros.
+  split; intro.
+  induction res.
+  - econstructor.
+    all: admit.
+  - inversion H.
+    unfold string_at_address in *.
+    unfold signed_string_to_Z in *.
+    unfold asn_strtoimax_lim in *.
+    unfold store_result in *.
+    unfold distance in *.
+    unfold vptr in *.
+    repeat break_match; try congruence.
+    unfold addr_ge, ptr_ge in *.
+    Admitted.
+    
+    
+(* Functional spec continued *)
 
 (* Moving towards implementation. Step 1: bounds on Z *)
 Section ZBoundsSpec.
@@ -155,97 +323,9 @@ Definition signed_string_to_int s :=
                     else string_to_int_plus s 
   end.
 
-(* Connecting different levels *)
-
-(* To relate the abstract spec we need to add assumption about memory *)
-Definition byte_of_int b := Byte.repr (Int.unsigned b).
-
-(* There is a string s at address str until fin *)
-(* Note: load returns value of type Vint, hence need a conversion from byte *)
-Definition string_at_address m str fin : option (list byte) :=
-  match distance m str fin with
-  | Some dist =>
-    let fix string_at_address m s str dist : option (list byte) :=
-        match dist with
-        | O => Some s
-        | S n => match load_addr Mint8signed m str with
-                | Some (Vint i) => string_at_address m
-                                                    ((byte_of_int i)::s)
-                                                    (str++) n
-                 | _ => None
-                 end
-        end in
-    string_at_address m nil str dist
-  | _ => None
-end.
-
 End IntSpec.
 
-Section RelationalSpec.
 
-Definition store_addr (chunk : memory_chunk) (m : mem) (a : addr) :=
-  match a with (b,ofs) => Mem.storev chunk m (Vptr b ofs) end.
-  
-  Inductive asn_strtoimax_lim_R m str fin intp : asn_strtox_result_e -> Prop :=
-    (* Input outside of supported numeric range *)
-  | ASN_STRTOX_ERROR_RANGE_R s z :
-      string_at_address m str fin = Some s ->
-      signed_string_to_Z s = Some z ->
-      (Int64.max_signed <= z)%Z \/ (z <= Int64.min_signed)%Z ->
-      asn_strtoimax_lim_R m str fin intp ASN_STRTOX_ERROR_RANGE
-    (* Invalid data encountered (e.g., "+-") *)
-  | ASN_STRTOX_ERROR_INVAL_R :
-      addr_ge m str fin = Some true ->
-      asn_strtoimax_lim_R m str fin intp ASN_STRTOX_ERROR_INVAL
-    (* More data expected (e.g. "+") *)
-  | ASN_STRTOX_EXPECT_MORE_R :
-      string_at_address m str fin = Some [plus_char] \/
-      string_at_address m str fin = Some [minus_char] ->
-      asn_strtoimax_lim_R m str fin intp ASN_STRTOX_EXPECT_MORE
-    (* Conversion succeded, but the string has extra stuff *)
-  | ASN_STRTOX_EXTRA_DATA_R s z m' :
-      string_at_address m str fin = Some s ->
-      signed_string_to_Z s = Some z ->
-      (Int64.min_signed <= z <= Int64.max_signed)%Z ->
-      (exists c, In c s /\ is_digit c = false) ->
-      store_addr Mint64 m intp (Vlong (Int64.repr z)) = Some m' -> 
-      asn_strtoimax_lim_R m str fin intp ASN_STRTOX_EXTRA_DATA
-      (* Conversion succeded *)
-  | ASN_STRTOX_OK_R s z m' :
-      string_at_address m str fin = Some s ->
-      signed_string_to_Z s = Some z ->
-      (Int64.min_signed <= z <= Int64.max_signed)%Z ->
-      store_addr Mint64 m intp (Vlong (Int64.repr z)) = Some m' -> 
-      asn_strtoimax_lim_R m str fin intp ASN_STRTOX_OK.  
-  
-End RelationalSpec.
-
-Theorem asn_strtoimax_lim_func_correct : forall m str fin fin' intp res,
-    asn_strtoimax_lim m str fin intp = Some res <->
-    (load_addr Mptr m fin = Some (vptr fin') /\
-     asn_strtoimax_lim_R m str fin' intp res.(return_type)).
-Proof.
-  intros.
-  destruct res.
-  destruct return_type.
-  split; intro.
-  - econstructor.
-    all: admit.
-  - inversion H.
-    unfold string_at_address in *.
-    unfold signed_string_to_Z in *.
-    unfold asn_strtoimax_lim in *.
-    unfold store_result in *.
-    unfold distance in *.
-    unfold vptr in *.
-    repeat break_match; try congruence.
-    unfold addr_ge, ptr_ge in *.
-    Admitted.
-    
-    
-    
-    
-  
     
     
   
